src/dvspec/dafny/att_spec_proofs/incomplete_proofs.dfy
@@ -12,6 +12,7 @@ include "../att_spec_proofs/dvn_next_invs_8_18.dfy"
 include "../att_spec_proofs/dvn_next_invs_19_26.dfy"
 include "../att_spec_proofs/common_proofs.dfy"
 include "../att_spec_proofs/fnc_invs_27_39.dfy"
+include "../specification/dvc_spec_axioms.dfy"
 
 module Incomplete_Proofs 
 {
@@ -29,219 +30,15 @@ module Incomplete_Proofs
     import opened Fnc_Invs_1_26    
     import opened Fnc_Invs_27_39
     import opened Common_Proofs
+    import opened DVCNode_Spec_Axioms
     
 
-    lemma {:axiom} axiom_inv37(
+    lemma {:axiom} axiom_lemma_pred_4_1_g_iii_c_dvn_next(
         dvn: DVState
     )    
-    ensures inv37(dvn)    
+    ensures pred_4_1_g_iii_c(dvn)    
 
 
     
-    lemma lemma_pred_4_1_g_iii_c_add_block_to_bn(
-        process: DVCNodeState,
-        block: BeaconBlock,
-        process': DVCNodeState        
-    )
-    requires add_block_to_bn.requires(process, block)
-    requires process' == add_block_to_bn(process, block)    
-    ensures process.latest_attestation_duty.isPresent()
-                == process'.latest_attestation_duty.isPresent();
-    ensures process.latest_attestation_duty.isPresent()
-                ==> ( process.latest_attestation_duty.safe_get()
-                        == process'.latest_attestation_duty.safe_get() )
-
-    { }
-
-    /*
-    lemma lemma_pred_4_1_g_iii_c_f_listen_for_attestation_shares(
-        process: DVCNodeState,
-        attestation_share: AttestationShare,
-        process': DVCNodeState
-    )
-    requires f_listen_for_attestation_shares.requires(process, attestation_share)
-    requires process' == f_listen_for_attestation_shares(process, attestation_share).state        
-    requires inv_g_iii_c_body_body(process)
-    ensures inv_g_iii_c_body_body(process')
-    {}
-
-    lemma lemma_pred_4_1_g_iii_c_f_start_next_duty(process: DVCNodeState, attestation_duty: AttestationDuty, process': DVCNodeState)
-    requires f_start_next_duty.requires(process, attestation_duty)
-    requires process' == f_start_next_duty(process, attestation_duty).state   
-    requires inv_g_iii_c_body_body(process)
-    ensures inv_g_iii_c_body_body(process')
-    { } 
-
-    lemma lemma_pred_4_1_g_iii_c_f_resend_attestation_share(
-        process: DVCNodeState,
-        process': DVCNodeState)
-    requires f_resend_attestation_share.requires(process)
-    requires process' == f_resend_attestation_share(process).state        
-    requires inv_g_iii_c_body_body(process)
-    ensures inv_g_iii_c_body_body(process')
-    { } 
-
-    lemma lemma_pred_4_1_g_iii_c_f_check_for_next_queued_duty(
-        process: DVCNodeState,
-        process': DVCNodeState
-    )
-    requires f_check_for_next_queued_duty.requires(process)
-    requires process' == f_check_for_next_queued_duty(process).state    
-    requires inv_g_iii_c_body_body(process)
-    ensures inv_g_iii_c_body_body(process')
-    decreases process.attestation_duties_queue
-    {
-        if  && process.attestation_duties_queue != [] 
-            && (
-                || process.attestation_duties_queue[0].slot in process.future_att_consensus_instances_already_decided
-                || !process.current_attestation_duty.isPresent()
-            )    
-        {            
-                if process.attestation_duties_queue[0].slot in process.future_att_consensus_instances_already_decided.Keys 
-                {
-                    var queue_head := process.attestation_duties_queue[0];
-                    var new_attestation_slashing_db := f_update_attestation_slashing_db(process.attestation_slashing_db, process.future_att_consensus_instances_already_decided[queue_head.slot]);
-                    var process_mod := process.(
-                        attestation_duties_queue := process.attestation_duties_queue[1..],
-                        future_att_consensus_instances_already_decided := process.future_att_consensus_instances_already_decided - {queue_head.slot},
-                        attestation_slashing_db := new_attestation_slashing_db,
-                        attestation_consensus_engine_state := updateConsensusInstanceValidityCheck(
-                            process.attestation_consensus_engine_state,
-                            new_attestation_slashing_db
-                        )                        
-                    );
-                    lemma_pred_4_1_g_iii_c_f_check_for_next_queued_duty(process_mod, process');
-                }
-                else
-                { 
-                    var process_mod := process.(
-                        attestation_duties_queue := process.attestation_duties_queue[1..]
-                    );     
-                    assert inv_g_iii_c_body_body(process_mod);
-
-                    lemma_pred_4_1_g_iii_c_f_start_next_duty(process_mod, process.attestation_duties_queue[0], process');
-                }
-        }
-        else
-        { 
-            assert process'.all_rcvd_duties == process.all_rcvd_duties;
-        }
-    }
-
-    lemma lemma_pred_4_1_g_iii_c_f_att_consensus_decided(
-        process: DVCNodeState,
-        id: Slot,
-        decided_attestation_data: AttestationData, 
-        process': DVCNodeState
-    )
-    requires f_att_consensus_decided.requires(process, id, decided_attestation_data)
-    requires process' == f_att_consensus_decided(process, id, decided_attestation_data).state         
-    requires inv_g_iii_c_body_body(process)
-    ensures inv_g_iii_c_body_body(process')
-    {
-        
-        var local_current_attestation_duty := process.current_attestation_duty.safe_get();
-        var attestation_slashing_db := f_update_attestation_slashing_db(process.attestation_slashing_db, decided_attestation_data);
-
-        var fork_version := bn_get_fork_version(compute_start_slot_at_epoch(decided_attestation_data.target.epoch));
-        var attestation_signing_root := compute_attestation_signing_root(decided_attestation_data, fork_version);
-        var attestation_signature_share := rs_sign_attestation(decided_attestation_data, fork_version, attestation_signing_root, process.rs);
-        var attestation_with_signature_share := AttestationShare(
-                aggregation_bits := get_aggregation_bits(local_current_attestation_duty.validator_index),
-                data := decided_attestation_data, 
-                signature := attestation_signature_share
-            ); 
-
-        var process := 
-            process.(
-                current_attestation_duty := None,
-                attestation_shares_to_broadcast := process.attestation_shares_to_broadcast[local_current_attestation_duty.slot := attestation_with_signature_share],
-                attestation_slashing_db := attestation_slashing_db,
-                attestation_consensus_engine_state := updateConsensusInstanceValidityCheck(
-                    process.attestation_consensus_engine_state,
-                    attestation_slashing_db
-                )
-            );
-
     
-        assert inv_g_iii_c_body_body(process);
-
-        var ret_check_for_next_queued_duty := f_check_for_next_queued_duty(process);
-        
-        lemma_pred_4_1_g_iii_c_f_check_for_next_queued_duty(process, ret_check_for_next_queued_duty.state);
-
-        assert process' == ret_check_for_next_queued_duty.state;        
-    } 
-    
-    lemma lemma_pred_4_1_g_iii_c_f_listen_for_new_imported_blocks(
-        process: DVCNodeState,
-        block: BeaconBlock,
-        process': DVCNodeState
-    )
-    requires f_listen_for_new_imported_blocks.requires(process, block)
-    requires process' == f_listen_for_new_imported_blocks(process, block).state        
-    requires inv_g_iii_c_body_body(process)
-    ensures inv_g_iii_c_body_body(process')
-    {
-        var new_consensus_instances_already_decided := f_listen_for_new_imported_blocks_helper_1(process, block);
-
-        var att_consensus_instances_already_decided := process.future_att_consensus_instances_already_decided + new_consensus_instances_already_decided;
-
-        var future_att_consensus_instances_already_decided := 
-            f_listen_for_new_imported_blocks_helper_2(process, att_consensus_instances_already_decided);
-
-        var process :=
-                process.(
-                    future_att_consensus_instances_already_decided := future_att_consensus_instances_already_decided,
-                    attestation_consensus_engine_state := stopConsensusInstances(
-                                    process.attestation_consensus_engine_state,
-                                    att_consensus_instances_already_decided.Keys
-                    ),
-                    attestation_shares_to_broadcast := process.attestation_shares_to_broadcast - att_consensus_instances_already_decided.Keys,
-                    rcvd_attestation_shares := process.rcvd_attestation_shares - att_consensus_instances_already_decided.Keys                    
-                );    
-        
-        assert inv_g_iii_c_body_body(process);
-
-        if process.current_attestation_duty.isPresent() && process.current_attestation_duty.safe_get().slot in att_consensus_instances_already_decided
-        {
-            var decided_attestation_data := att_consensus_instances_already_decided[process.current_attestation_duty.safe_get().slot];
-            var new_attestation_slashing_db := f_update_attestation_slashing_db(process.attestation_slashing_db, decided_attestation_data);
-            var process := process.(
-                current_attestation_duty := None,
-                attestation_slashing_db := new_attestation_slashing_db,
-                attestation_consensus_engine_state := updateConsensusInstanceValidityCheck(
-                    process.attestation_consensus_engine_state,
-                    new_attestation_slashing_db
-                )                
-            );
-            
-            assert inv_g_iii_c_body_body(process);
-
-            lemma_pred_4_1_g_iii_c_f_check_for_next_queued_duty(process, process');
-        }
-        else
-        {               
-            assert inv_g_iii_c_body_body(process);
-        }
-    } 
-
-    lemma lemma_pred_4_1_g_iii_c_f_serve_attestation_duty(
-        process: DVCNodeState,
-        attestation_duty: AttestationDuty,
-        process': DVCNodeState
-    )  
-    requires f_serve_attestation_duty.requires(process, attestation_duty)
-    requires process' == f_serve_attestation_duty(process, attestation_duty).state
-    requires inv_g_iii_c_body_body(process)
-    ensures inv_g_iii_c_body_body(process')
-    {
-        var process_mod := process.(
-                attestation_duties_queue := process.attestation_duties_queue + [attestation_duty],
-                all_rcvd_duties := process.all_rcvd_duties + {attestation_duty}
-            );        
-        
-        lemma_pred_4_1_g_iii_c_f_check_for_next_queued_duty(process_mod, process');        
-    } 
-    */
 }
